platform/XmlSearch.v
@@ -44,10 +44,12 @@ Fixpoint allCdatas (p : pat) : list (string * string) :=
 (** * Compiling patterns into Bedrock chunks *)
 
 Section Pat.
+  (* Do all start-length pairs in a list denote valid spans in a string of length "len"? *)
   Definition inBounds (cdatas : list (string * string)) (V : vals) :=
     List.Forall (fun p => wordToNat (V (fst p)) + wordToNat (V (snd p)) <= wordToNat (V "len"))%nat
     cdatas.
 
+  (* Are all saved positions in a list valid pointers within a string of a given length? *)
   Definition stackOk (ls : list W) (len : W) :=
     List.Forall (fun x => x <= len) ls.
 
@@ -84,34 +86,56 @@ Section Pat.
       * [| wordToNat (V start) + wordToNat R <= wordToNat (V "len") |]%nat
     POST[_] array8 bs (V "buf").
 
+  (* Alternate sequencing operator, which generates twistier code but simpler postconditions and VCs *)
+  Definition SimpleSeq (ch1 ch2 : chunk) : chunk := fun ns res =>
+    Structured nil (fun im mn H => Seq_ H (toCmd ch1 mn H ns res) (toCmd ch2 mn H ns res)).
+
+  Infix ";;" := SimpleSeq : SP_scope.
+
+  (* Workhorse pattern compilation function, taking as input:
+   * p: an XML pattern to compile
+   * level: tree depth at which this pattern is applied (starts at 1 for top-level pattern)
+   * cdatas: list of start-length pairs denoting spans within the string we match against,
+   *         set by earlier successfull matches of subpatterns
+   * onSuccess: continuation code to run when the pattern matches fully
+   *)
   Fixpoint Pat' (p : pat) (level : nat) (cdatas : list (string * string))
     (onSuccess : chunk) : chunk :=
     match p with
       | Cdata start len =>
+        (* Read next token. *)
         "res" <-- Call "xml_lex"!"next"("buf", "lex")
         [inv cdatas];;
 
+        (* What type of token is it? *)
         If ("res" = 2) {
           (* This is indeed CDATA!  Save the position and signal success. *)
           start <-- Call "xml_lex"!"tokenStart"("lex")
           [invP cdatas];;
 
-          len <-- Call "xml_lex"!"tokenStart"("lex")
+          len <-- Call "xml_lex"!"tokenLength"("lex")
           [invL cdatas start];;
 
           onSuccess
         } else {
+          (* It's not CDATA.  Pattern doesn't match. *)
           Skip
         }
 
       | Tag tag inner =>
+        (* Initialize a variable storing the tree depth of our current position.
+         * We'll consult this variable to see when we're at the proper depth for matching
+         * the current pattern. *)
         "level" <- level;;
 
+        (* Loop until level drops below the starting level (after which the pattern never applies again). *)
         [inv cdatas]
         While ("level" >= level) {
+          (* Lex next token. *)
           "res" <-- Call "xml_lex"!"next"("buf", "lex")
           [inv cdatas];;
 
+          (* What type of token is it? *)
           If ("res" = 1) {
             (* Open tag -- does it match? *)
             "level" <- "level" + 1;;
@@ -120,12 +144,14 @@ Section Pat.
               (* We've descended too deep, so this position doesn't qualify. *)
               Skip
             } else {
+              (* We may have a match!  First, grab the boundaries of the matching string. *)
               "tagStart" <-- Call "xml_lex"!"tokenStart"("lex")
               [invP cdatas];;
 
               "tagLen" <-- Call "xml_lex"!"tokenStart"("lex")
               [invL cdatas "tagStart"];;
 
+              (* Now check if the tag name here matches the name from the pattern. *)
               StringEq "buf" "len" "tagStart" "matched" tag
               (A := unit)
               (fun _ V => xmlp (V "len") (V "lex")
@@ -134,8 +160,10 @@ Section Pat.
                 * [| inBounds cdatas V |])%Sep;;
 
               If ("matched" = 0) {
+                (* Nope, not equal. *)
                 Skip
               } else {
+                (* Equal!  Continue with the nested pattern. *)
                 Pat' inner (S level) cdatas onSuccess
               }
             }
@@ -148,6 +176,7 @@ Section Pat.
                 (* Done parsing.  Force exit from the loop. *)
                 "level" <- 0
               } else {
+                (* Ignore any other kind of token. *)
                 Skip
               }
             }
@@ -157,6 +186,7 @@ Section Pat.
       | Both p1 p2 =>
         (* Warning: shameless reuse here of variables for new purposes *)
 
+        (* Get the current position, which we will save to return to later. *)
         "tagLen" <-- Call "xml_lex"!"position"("lex")
         [Al bs, Al ls,
           PRE[V, R] array8 bs (V "buf") * xmlp (V "len") (V "lex")
@@ -165,28 +195,37 @@ Section Pat.
             * [| stackOk ls (V "len") |]
           POST[_] array8 bs (V "buf")];;
 
+        (* Allocate a new entry for the position stack. *)
         "tagStart" <-- Call "malloc"!"malloc"(0, 2)
         [Al bs, Al ls,
           PRE[V, R] array8 bs (V "buf") * xmlp (V "len") (V "lex")
             * sll ls (V "stack") * [| V "tagLen" <= V "len" |]%word
-            * [| R <> 0 |] * [| freeable R 2 |]
+            * R =?> 2 * [| R <> 0 |] * [| freeable R 2 |]
             * [| length bs = wordToNat (V "len") |] * [| inBounds cdatas V |]
             * [| stackOk ls (V "len") |]
           POST[_] array8 bs (V "buf")];;
 
+        (* Save the current position in this entry, then push it onto the stack. *)
         "tagStart" *<- "tagLen";;
-        "tagStart" *<- "stack";;
+        "tagStart"+4 *<- "stack";;
         "stack" <- "tagStart";;
 
+        (* Try matching the first pattern. *)
         Pat' p1 level cdatas
-        (If ("stack" = 0) {
+        ((* Make sure the stack is nonempty afterward.
+          * Only buggy code here could lead to that outcome, but we aren't verifying at that level
+          * of detail yet, so we use a run-time check. *)
+        If ("stack" = 0) {
+          (* We hope this case is impossible. *)
           Call "sys"!"abort"()
           [PREonly[_] [| False |]]
         } else {
+          (* Stack nonempty!  Pop position off of stack (into "tagLen"). *)
           "tagLen" <-* "stack";;
           "tagStart" <- "stack";;
           "stack" <-* "stack"+4;;
 
+          (* Free the popped stack entry. *)
           Call "malloc"!"free"(0, "tagStart", 2)
           [Al bs, Al ls,
             PRE[V] array8 bs (V "buf") * xmlp (V "len") (V "lex")
@@ -195,22 +234,24 @@ Section Pat.
               * [| stackOk ls (V "len") |]
           POST[_] array8 bs (V "buf")];;
 
+          (* Restore the position we popped. *)
           Call "xml_lex"!"setPosition"("lex", "tagLen")
           [inv cdatas];;
 
+          (* Now try matching the second pattern from the same initial position. *)
           Pat' p2 level (allCdatas p1 ++ cdatas)
           onSuccess
         })
     end%SP.
 
   Notation baseVars := ("buf" :: "len" :: "lex" :: "res"
-    :: "tagStart" :: "tagLen" :: "matched" :: nil).
+    :: "tagStart" :: "tagLen" :: "matched" :: "stack" :: nil).
 
   Definition noConflict pt := List.Forall (fun p => ~In (fst p) baseVars /\ ~In (snd p) baseVars
     /\ ~freeVar pt (fst p) /\ ~freeVar pt (snd p)).
 
   Notation PatVcs' p cdatas onSuccess := (fun ns =>
-    (~In "rp" ns) :: In "buf" ns :: In "len" ns :: In "lex" ns :: In "res" ns :: In "matched" ns
+    (~In "rp" ns) :: incl baseVars ns
     :: (forall x, freeVar p x -> In x ns /\ ~In x baseVars /\ x <> "rp")
     :: wf p
     :: noConflict p cdatas
@@ -231,7 +272,15 @@ Section Pat.
     induction 1; inversion 1; eauto.
   Qed.
 
+  Lemma incl_peel : forall A (x : A) ls ls',
+    incl (x :: ls) ls'
+    -> In x ls' /\ incl ls ls'.
+    unfold incl; intuition.
+  Qed.
+
   Ltac deDouble := repeat match goal with
+                            | [ H : incl nil _ |- _ ] => clear H
+                            | [ H : incl _ _ |- _ ] => apply incl_peel in H; destruct H
                             | [ H : forall x, x = _ \/ x = _ -> _ |- _ ] =>
                               generalize (H _ (or_introl _ eq_refl)); intro;
                                 specialize (H _ (or_intror _ eq_refl))
@@ -276,6 +325,15 @@ Section Pat.
 
   Opaque mult.
 
+  Lemma stackOk_cons : forall w len ws,
+    w <= len
+    -> stackOk ws len
+    -> stackOk (w :: ws) len.
+    constructor; auto.
+  Qed.
+
+  Local Hint Immediate stackOk_cons.
+
   Definition PatR (p : pat) (level : nat) (cdatas : list (string * string))
     (onSuccess : chunk) : chunk.
     refine (WrapC (Pat' p level cdatas onSuccess)
@@ -284,15 +342,25 @@ Section Pat.
       (PatVcs' p cdatas onSuccess)
       _ _).
 
-    generalize dependent cdatas; generalize dependent level; induction p;
-      (wrap0; deDouble; try solve [ app; simp ];
-        simp; evalu; descend; (try rewrite inBounds_sel; descend; step auto_ext; eauto; inBounds || finish)).
+    generalize dependent onSuccess; generalize dependent cdatas; generalize dependent level; induction p;
+      wrap0; deDouble.
+
+    Ltac t := simp; evalu; descend; (try rewrite inBounds_sel; descend; step SinglyLinkedList.hints;
+      try step SinglyLinkedList.hints; eauto; inBounds || finish).
+
+    try solve [ app; simp ]; t.
+    try solve [ app; simp ]; t.
+
+    app.
+    t.
+    t.
+    admit.
 
     admit.
   Defined.
 
-  Notation PatVcs p := (fun ns =>
-    (~In "rp" ns) :: In "buf" ns :: In "len" ns :: In "lex" ns :: In "res" ns :: In "matched" ns
+  Notation PatVcs p onSuccess := (fun ns =>
+    (~In "rp" ns) :: incl baseVars ns
     :: (forall x, freeVar p x -> In x ns /\ ~In x baseVars)
     :: wf p
     :: (forall specs im mn H res pre st,
@@ -300,11 +368,11 @@ Section Pat.
       -> interp specs (invar true (fun w => w) ns res st))
     :: nil).
 
-  Definition Pat (p : pat) : chunk.
-    refine (WrapC (PatR p 1 nil)
+  Definition Pat (p : pat) (onSuccess : chunk) : chunk.
+    refine (WrapC (PatR p 1 nil onSuccess)
       invar
       invar
-      (PatVcs p)
+      (PatVcs p onSuccess)
       _ _).
 
     wrap0; simp; descend;
